src/Pyrosome/Tools/EGraph/Theorems.v
@@ -603,15 +603,13 @@ Section WithVar.
                 | None => True
                 end.
     
-    Arguments model_satisfies_rule {idx symbol}%type_scope {idx_map}%function_scope m r.
 
-    Lemma sequent_of_states_sound A B m i1 s1 Post_i Post Post2 Post_i2
+    Lemma sequent_of_states_sound A B m i1 s1 Post Post2
       (s2 : A -> state (instance _) B)
-      : state_sound_for_model m i1 s1 Post_i Post ->
+      : state_sound_for_model m i1 s1 Post ->
         (forall a i2, map.extends i2 i1 ->
-                      (Post_i i2) ->
                       Post i2 a ->
-                      state_sound_for_model m i2 (s2 a) Post_i2 Post2) ->
+                      state_sound_for_model m i2 (s2 a) Post2) ->
         model_satisfies_rule m (sequent_of_states s1 s2).
     Proof.
       intros.
